src/theories/N.v
@@ -1,0 +1,78 @@
+From Equations Require Import Equations.
+Require Import Coq.Program.Equality.
+Require Import Coq.Lists.List.
+
+Require Import MirrorSolve.FirstOrder.
+Require Import MirrorSolve.HLists.
+
+Import ListNotations.
+Import HListNotations.
+
+Require Import Coq.ZArith.BinInt.
+
+Section NFOL.
+  Inductive sorts: Set :=
+  | NS
+  | BS.
+
+  Inductive funs: arity sorts -> sorts -> Type :=
+  | NLit: forall (n: nat), funs [] NS
+  | BLit: forall (b: bool), funs [] BS
+  | Sub: funs [NS; NS] NS
+  | Plus: funs [NS; NS] NS
+  | Mul: funs [NS; NS] NS
+  | Div: funs [NS; NS] NS
+  | Mod: funs [NS; NS] NS
+  | Lte: funs [NS; NS] BS
+  | Lt: funs [NS; NS] BS
+  | Gte: funs [NS; NS] BS
+  | Gt: funs [NS; NS] BS.
+
+
+  Inductive rels: arity sorts -> Type :=.
+
+  Definition sig: signature :=
+    {| sig_sorts := sorts;
+      sig_funs := funs;
+      sig_rels := rels |}.
+
+  Definition fm ctx := FirstOrder.fm sig ctx.
+  Definition tm ctx := FirstOrder.tm sig ctx.
+
+  Definition mod_sorts (s: sig_sorts sig) : Type :=
+    match s with
+    | NS => nat
+    | BS => bool
+    end.
+
+  Obligation Tactic := idtac.
+  Equations 
+    mod_fns params ret (f: sig_funs sig params ret) (args: HList.t mod_sorts params) 
+    : mod_sorts ret :=
+    { mod_fns _ _ (BLit b) _ := b;
+      mod_fns _ _ (NLit n) _ := n;
+      mod_fns _ _ Sub (l ::: r ::: _) := Nat.sub l r;
+      mod_fns _ _ Plus (l ::: r ::: _) := Nat.add l r;
+      mod_fns _ _ Mul (l ::: r ::: _) := Nat.mul l r;
+      mod_fns _ _ Div (l ::: r ::: _) := Nat.div l r;
+      mod_fns _ _ Mod (l ::: r ::: _) := Nat.modulo l r;
+      mod_fns _ _ Lte (l ::: r ::: _) := Nat.leb l r;
+      mod_fns _ _ Lt (l ::: r ::: _) := Nat.ltb l r;
+      mod_fns _ _ Gte (l ::: r ::: _) := Nat.leb r l;
+      mod_fns _ _ Gt (l ::: r ::: _) := Nat.ltb l r;
+    }.
+
+  Definition mod_rels params
+    (args: sig_rels sig params)
+    (env: HList.t mod_sorts params) : Prop :=
+    match args with
+    end.
+
+  Definition fm_model : model sig := {|
+    FirstOrder.mod_sorts := mod_sorts;
+    FirstOrder.mod_fns := mod_fns;
+    FirstOrder.mod_rels := mod_rels;
+  |}.
+
+End NFOL.
+
