src/theories/N2Z.v
@@ -1,0 +1,179 @@
+From Equations Require Import Equations.
+Require Import Coq.Program.Equality.
+Require Import Coq.Lists.List.
+
+Require Import MirrorSolve.FirstOrder.
+Require Import MirrorSolve.HLists.
+
+Import ListNotations.
+Import HListNotations.
+
+Require Import Coq.ZArith.BinInt.
+
+Require Import MirrorSolve.N.
+Require Import MirrorSolve.Z.
+
+Set Universe Polymorphism. 
+
+Section N2Z.
+
+  
+
+  Definition n2z_sort (ns: N.sorts) : Z.sorts := 
+    match ns with 
+    | NS => ZS
+    | N.BS => BS
+    end.
+
+  Fixpoint n2z_arr (na: arity N.sorts) : arity Z.sorts :=
+    match na with 
+    | nil => nil
+    | ns :: na' => n2z_sort ns :: (n2z_arr na')
+    end.
+
+  Equations n2z_fun {arr : arity (sig_sorts N.sig)} {srt: sig_sorts N.sig} (nf: sig_funs N.sig arr srt) : sig_funs sig (n2z_arr arr) (n2z_sort srt) :=
+  {
+    n2z_fun (NLit n) := ZLit (Z.of_nat n);
+    n2z_fun (N.BLit b) := BLit b;
+    n2z_fun N.Sub := Z.Sub;
+    n2z_fun N.Plus := Z.Plus;
+    n2z_fun N.Mul := Z.Mul;
+    n2z_fun N.Div := Z.Div;
+    n2z_fun N.Mod := Z.Mod;
+    n2z_fun N.Gt := Z.Gt;
+    n2z_fun N.Gte := Z.Gte;
+    n2z_fun N.Lt := Z.Lt;
+    n2z_fun N.Lte := Z.Lte;
+  }.
+
+  Definition n2z_rel {arr: arity (sig_sorts N.sig)} (r: sig_rels N.sig arr) : sig_rels sig (n2z_arr arr) := 
+    match r with end.
+
+  Equations n2z_mv {srt} (v: N.mod_sorts srt) : Z.mod_sorts (n2z_sort srt) := 
+  {
+    @n2z_mv N.NS n := Z.of_nat n;
+    @n2z_mv N.BS b := b;
+  }.
+
+  
+
+  Program Definition n2z_func : @theory_functor N.sig Z.sig N.fm_model Z.fm_model := {|
+    fmap_sorts := n2z_sort;
+    fmap_arity := n2z_arr;
+    fmap_funs := @n2z_fun;
+    fmap_rels := @n2z_rel;
+    fmap_mv := @n2z_mv;
+  |}.
+
+  (* Notation fmap_ctx := (@fmap_ctx n2z_func). *)
+
+  Notation fmap_ctx' := (fmap_ctx _ _ _ _ n2z_func).
+
+  Equations n2z_fun_arrs {c arr srt} 
+    (f: N.funs arr srt) 
+    (args: HList.t (fun srt' : N.sorts => FirstOrder.tm sig (fmap_ctx' c) (n2z_sort srt')) arr) : 
+    HList.t (FirstOrder.tm sig (fmap_ctx' c)) (n2z_arr arr) := 
+  {
+    n2z_fun_arrs (NLit n) _ := hnil;
+    n2z_fun_arrs (N.BLit b) _ := hnil;
+    n2z_fun_arrs N.Sub (x ::: y ::: _) := _;
+    n2z_fun_arrs N.Plus (x ::: y ::: _) := _;
+    n2z_fun_arrs N.Mul (x ::: y ::: _) := _;
+    n2z_fun_arrs N.Div (x ::: y ::: _) := _;
+    n2z_fun_arrs N.Mod (x ::: y ::: _) := _;
+    n2z_fun_arrs N.Gt (x ::: y ::: _) := _;
+    n2z_fun_arrs N.Gte (x ::: y ::: _) := _;
+    n2z_fun_arrs N.Lt (x ::: y ::: _) := _;
+    n2z_fun_arrs N.Lte (x ::: y ::: _) := _;
+  }.
+  Next Obligation.
+    exact (x ::: y ::: hnil).  (* I don't know why but I can't put this in the body of the definition? *)
+  Defined.
+  Next Obligation. exact (x ::: y ::: hnil). Defined.
+  Next Obligation. exact (x ::: y ::: hnil). Defined.
+  Next Obligation. exact (x ::: y ::: hnil). Defined.
+  Next Obligation. exact (x ::: y ::: hnil). Defined.
+  Next Obligation. exact (x ::: y ::: hnil). Defined.
+  Next Obligation. exact (x ::: y ::: hnil). Defined.
+  Next Obligation. exact (x ::: y ::: hnil). Defined.
+  Next Obligation. exact (x ::: y ::: hnil). Defined.
+
+  Definition n2z_rel_arrs {c arr} (rel: N.rels arr) (args: HList.t (fun srt' : N.sorts => FirstOrder.tm sig (fmap_ctx' c) (n2z_sort srt')) arr) 
+    : HList.t (FirstOrder.tm sig (fmap_ctx' c)) (n2z_arr arr) := 
+  match rel with end.
+
+  Program Definition n2z_forall_op {c} {srt: sig_sorts N.sig} (f: FirstOrder.fm sig (fmap_ctx' (CSnoc N.sig c srt))) : FirstOrder.fm sig (fmap_ctx' (CSnoc N.sig c srt)) := 
+    match srt with 
+    | N.BS => f
+    | N.NS => 
+      FImpl (FEq (s := Z.BS) 
+        (TFun _ (@BLit true) hnil) 
+        (TFun _ Z.Gte ((TVar (VHere _ _ _)) ::: (TFun _ (@ZLit 0%Z) hnil) ::: hnil))
+      ) f
+    end.
+
+  (* Lemma n2z_tm_inj: 
+  forall 
+    (srt : sig_sorts N.sig) (c : ctx N.sig)
+    (v : valu N.sig N.fm_model c) (t t' : FirstOrder.tm N.sig c srt),
+    interp_tm v t = interp_tm v t' <->
+    interp_tm
+      (fmap_valu N.sig sig n2z_sort N.fm_model fm_model (@n2z_mv) v)
+      (fmap_tm N.sig sig n2z_sort n2z_arr (@n2z_fun) (@n2z_fun_arrs) t) =
+    interp_tm
+      (fmap_valu N.sig sig n2z_sort N.fm_model fm_model (@n2z_mv) v)
+      (fmap_tm N.sig sig n2z_sort n2z_arr (@n2z_fun) (@n2z_fun_arrs) t').
+  Proof.
+    intros.
+    dependent induction t using tm_ind';
+    dependent destruction t';
+    simpl.
+    - inversion v0; subst;
+      dependent destruction v;
+      autorewrite with interp_tm.
+
+      autorewrite with fmap_valu.
+      unfold @n2
+      simpl.
+
+      inversion v;  *)
+
+  
+  Program Definition n2z_wf : functor_wf _ _ _ _ n2z_func (@n2z_fun_arrs) (@n2z_rel_arrs) (@n2z_forall_op) := {|
+    interp_tm_inj := _;
+    fmap_rel_equi := _;
+    interp_fmap_forall_equi := _;
+  |}.
+  Admit Obligations.
+
+  Lemma n2z_corr: 
+    forall (c : ctx N.sig) (v : valu N.sig N.fm_model c) (f : FirstOrder.fm N.sig c),
+      interp_fm v f <->
+      interp_fm (fmap_valu N.sig sig N.fm_model fm_model n2z_func v)
+        (fmap_fm N.sig sig N.fm_model fm_model n2z_func 
+            (@n2z_fun_arrs) (@n2z_rel_arrs) (@n2z_forall_op) f).
+  Proof.
+    eapply fmap_corr.
+    exact n2z_wf.
+  Qed.
+
+
+  Lemma nat_eq_refl : 
+    interp_fm (sig := N.sig) (VEmp _ N.fm_model) (FForall (sig :=  N.sig) NS (FForall (sig :=  N.sig) NS (FEq 
+      (TFun N.sig N.Plus (
+        ((TVar (VHere _ _ _)) ::: (TVar (VThere _ _ _ _ (VHere _ _ _)) ::: hnil))
+      ))
+      (TFun N.sig N.Plus (
+        ((TVar (VHere _ _ _)) ::: (TVar (VThere _ _ _ _ (VHere _ _ _)) ::: hnil))
+      ))
+    ))).
+  Proof.
+    eapply n2z_corr.
+    match goal with 
+    | |- interp_fm ?v ?f => 
+      set (v' := v);
+      set (f' := f)
+    end.
+    vm_compute in f'.
+  Admitted.
+End N2Z.
